Tests/All.lean
@@ -2,8 +2,10 @@ import Tests.Lexer
 import Tests.Golden
 import Tests.IR
 import Tests.PublicInterface
+import Tests.Diagnostic
 
 def main : IO Unit := do
   lexerMain
   irMain
+  diagnosticMain
   goldenMain
